src/Pyrosome/Lang/Levels.v
@@ -1,0 +1,186 @@
+Require Import Datatypes.String Lists.List.
+Import ListNotations.
+Open Scope string.
+Open Scope list.
+From Utils Require Import Utils.
+From Pyrosome Require Import
+  Theory.Core Elab.Elab
+  Elab.PreRule
+  Tools.ComputeWf
+  Tools.Matches Tools.EGraph.TypeInference
+  Tools.EGraph.ComputeWf
+  Tools.EGraph.Automation
+  Tools.Interactive.
+
+From Pyrosome.Lang Require Import
+  Subst SubstEqnGen
+  Pi Sigma.
+
+Require Coq.derive.Derive.
+
+Import Core.Notations.
+Import PreRule.Notations.
+
+(*TODO: move to Automation.v*)
+Ltac auto_elab' reversible do_check :=
+  setup_elab_lang;
+  repeat
+    ([>unshelve (solve
+                   [ break_elab_rule; (*try decompose_sort_eq;*)
+                     try apply eq_term_refl;
+                     try Automation.by_reduction' reversible do_check;
+                     cleanup_auto_elab ]);
+      try apply eq_term_refl; cleanup_auto_elab
+     | .. ]).
+
+
+Ltac auto_elab :=
+  auto_elab' (fun _ : string * Rule.rule string => true) idtac.
+
+Ltac auto_elab_no_check :=
+  auto_elab' (fun _ : string * Rule.rule string => true) fail.
+
+
+Derive levels
+       SuchThat (wf_lang (levels : lang))
+       As levels_wf.
+Proof.
+  setup_lang_interactive.
+
+  elab_rule {[r
+      -----------------------------------------------
+      #"lvl" srt
+    ]}%prerule
+    (@nil (string* list string)).  
+  elab_rule {[r
+      -----------------------------------------------
+      #"l0" : #"lvl"
+    ]}%prerule
+    (@nil (string* list string)).
+  elab_rule {[r "l" : #"lvl"
+      -----------------------------------------------
+      #"lS" "l" : #"lvl"
+    ]}%prerule
+    (@nil (string* list string)).
+  elab_rule {[r  "l1" : #"lvl",  "l2" : #"lvl"
+      -----------------------------------------------
+      #"<" "l1" "l2" srt
+    ]}%prerule
+    (@nil (string* list string)).  
+  elab_rule {[r "l" : #"lvl"
+      -----------------------------------------------
+      #"<0" : #"<" #"l0" (#"lS" "l")
+    ]}%prerule
+    (@nil (string* list string)).
+  elab_rule {[r "l" : #"lvl"
+      -----------------------------------------------
+      #"<S" : #"<" "l" (#"lS" "l")
+    ]}%prerule
+    (@nil (string* list string)).
+  elab_rule {[r "l1" : #"lvl", "l2" : #"lvl", "p" : #"<" "l1" "l2"
+      -----------------------------------------------
+      #"<S_cong" "p" : #"<" (#"lS" "l1") (#"lS" "l2")
+    ]}%prerule
+    (@nil (string* list string)).
+  elab_rule {[r "l1" : #"lvl",
+          "l2" : #"lvl",
+            "p1" : #"<" "l1" "l2",
+          "l3" : #"lvl",
+            "p2" : #"<" "l2" "l3"
+      -----------------------------------------------
+      #"<trans" "p1" "p2" : #"<" "l1" "l3"
+    ]}%prerule
+    (@nil (string* list string)).
+  elab_rule {[r "l1" : #"lvl",
+          "l2" : #"lvl",
+            "p1" : #"<" "l1" "l2",
+            "p2" : #"<" "l1" "l2"
+      ----------------------------------------------- ("<irr")
+      #"p1" = "p2" : #"<" "l1" "l3"
+    ]}%prerule
+    (@nil (string* list string)).
+  apply wf_lang_nil.
+Unshelve.
+1:shelve.
+1:vm_compute; reflexivity.
+Qed.
+#[export] Hint Resolve levels_wf : elab_pfs.
+
+Definition levels_injectivity :=
+  [("<", ["l2"; "l1"]);("lS", ["l"]); ("l0", []);
+   ("lvl", [])].
+
+Require Import Pyrosome.Compilers.Parameterizer.
+
+
+#[local] Definition subst_leveled' :=
+    let ps := (elab_param "l" (subst_lang)
+                 [(*("env", None);
+                   ("sub", None);*)
+                ("exp",Some 1);
+                ("ty", Some 0)]) in
+  parameterize_lang "l" {{s #"lvl"}}
+    ps subst_lang.
+
+Definition subst_leveled :=
+  Eval vm_compute in subst_leveled'.
+
+Ltac compute_wf_lang ::=
+  apply compute_wf_lang_sound
+    with (fuel := 100)
+         (rebuild_fuel := 100)
+         (saturation_fuel := 10)
+         (filter:=Automation.filter_rules)
+         (reversible:=Automation.filter_rules);
+  [ prove_from_known_elabs | vm_compute; reflexivity].
+
+Ltac compute_wf_lang_no_check :=
+  apply compute_wf_lang_sound
+    with (fuel := 100)
+         (rebuild_fuel := 100)
+         (saturation_fuel := 10)
+         (filter:=Automation.filter_rules)
+         (reversible:=Automation.filter_rules);
+  [ prove_from_known_elabs | vm_cast_no_check I].
+
+Lemma subst_leveled_wf
+  : wf_lang_ext levels subst_leveled.
+Proof.
+  compute_wf_lang_no_check.
+Qed.
+#[export] Hint Resolve subst_leveled_wf : elab_pfs.
+
+
+(*TODO: parameterize subst injectivity programmatically?
+  When should the parameter be injective? always?
+ *)
+Definition subst_injectivity :=
+  [("hd", ["A"; "l"; "G"]); ("wkn", ["A"; "l"; "G"]);
+   ("snoc", ["v"; "A"; "l"; "g"; "G'"; "G"]); ("ext", ["A"; "G"]);
+   ("forget", ["G"]); ("emp", []); ("ty", ["l";"G"]); ("ty_subst", ["l";"G"]);
+   ("exp_subst", ["l";"G"]); ("exp", ["A"; "l"; "G"]);
+   ("cmp", ["G3"; "G1"]); ("id", ["G"]); ("sub", ["G'"; "G"]); ("env", [])].
+
+#[local] Definition pi_leveled' :=
+    let ps := (elab_param "l" (pi++subst_lang)
+                 [(*("env", None);
+                   ("sub", None);*)
+                ("exp",Some 1);
+                ("ty", Some 0)]) in
+  parameterize_lang "l" {{s #"lvl"}}
+    ps pi.
+
+Definition pi_leveled :=
+  Eval vm_compute in pi_leveled'.
+
+
+Lemma pi_leveled_wf
+  : wf_lang_ext (subst_leveled++levels) pi_leveled.
+Proof.
+  compute_wf_lang_no_check.
+Qed.
+#[export] Hint Resolve pi_leveled_wf : elab_pfs.
+
+(*
+TODO: level promotion constructs
+*)
